tacenta-proofs/translation/Translation/TacentaSpqr.lean
@@ -140,6 +140,15 @@ def U8.Insts.ZeroizeDefaultIsZeroes : zeroize.DefaultIsZeroes Std.U8 := {
   coredefaultDefaultInst := core.default.DefaultU8
 }
 
+/-- Trait implementation: [zeroize::{impl zeroize::DefaultIsZeroes for u64}]
+    Source: '/cargo/registry/src/index.crates.io-1949cf8c6b5b557f/zeroize-1.9.0/src/lib.rs', lines 282:10-282:40
+    Name pattern: [zeroize::DefaultIsZeroes<u64>] -/
+@[reducible, rust_trait_impl "zeroize::DefaultIsZeroes<u64>"]
+def U64.Insts.ZeroizeDefaultIsZeroes : zeroize.DefaultIsZeroes Std.U64 := {
+  coremarkerCopyInst := core.marker.CopyU64
+  coredefaultDefaultInst := core.default.DefaultU64
+}
+
 /-- [zeroize::{impl zeroize::Zeroize for [Z; N]}::zeroize]:
     Source: '/cargo/registry/src/index.crates.io-1949cf8c6b5b557f/zeroize-1.9.0/src/lib.rs', lines 346:4-346:25
     Name pattern: [zeroize::{zeroize::Zeroize<[@Z; @N]>}::zeroize]
@@ -156,6 +165,43 @@ axiom Array.Insts.ZeroizeZeroize.zeroize
 def Array.Insts.ZeroizeZeroize {Z : Type} (N : Std.Usize) (ZeroizeInst :
   zeroize.Zeroize Z) : zeroize.Zeroize (Array Z N) := {
   zeroize := Array.Insts.ZeroizeZeroize.zeroize ZeroizeInst
+}
+
+/-- [zeroize::{impl zeroize::Zeroize for core::option::Option<Z>}::zeroize]:
+    Source: '/cargo/registry/src/index.crates.io-1949cf8c6b5b557f/zeroize-1.9.0/src/lib.rs', lines 369:4-369:25
+    Name pattern: [zeroize::{zeroize::Zeroize<core::option::Option<@Z>>}::zeroize]
+    Visibility: public -/
+@[rust_fun "zeroize::{zeroize::Zeroize<core::option::Option<@Z>>}::zeroize"]
+axiom core.option.Option.Insts.ZeroizeZeroize.zeroize
+  {Z : Type} (ZeroizeInst : zeroize.Zeroize Z) : Option Z → Result (Option Z)
+
+/-- Trait implementation: [zeroize::{impl zeroize::Zeroize for core::option::Option<Z>}]
+    Source: '/cargo/registry/src/index.crates.io-1949cf8c6b5b557f/zeroize-1.9.0/src/lib.rs', lines 365:0-367:15
+    Name pattern: [zeroize::Zeroize<core::option::Option<@Z>>] -/
+@[reducible, rust_trait_impl "zeroize::Zeroize<core::option::Option<@Z>>"]
+def core.option.Option.Insts.ZeroizeZeroize {Z : Type} (ZeroizeInst :
+  zeroize.Zeroize Z) : zeroize.Zeroize (Option Z) := {
+  zeroize := core.option.Option.Insts.ZeroizeZeroize.zeroize ZeroizeInst
+}
+
+/-- [zeroize::{impl zeroize::Zeroize for (A, B)}::zeroize]:
+    Source: '/cargo/registry/src/index.crates.io-1949cf8c6b5b557f/zeroize-1.9.0/src/lib.rs', lines 496:12-496:33
+    Name pattern: [zeroize::{zeroize::Zeroize<(@A, @B)>}::zeroize]
+    Visibility: public -/
+@[rust_fun "zeroize::{zeroize::Zeroize<(@A, @B)>}::zeroize"]
+axiom Pair.Insts.ZeroizeZeroize.zeroize
+  {A : Type} {B : Type} (ZeroizeInst : zeroize.Zeroize A) (ZeroizeInst1 :
+  zeroize.Zeroize B) :
+  (A × B) → Result (A × B)
+
+/-- Trait implementation: [zeroize::{impl zeroize::Zeroize for (A, B)}]
+    Source: '/cargo/registry/src/index.crates.io-1949cf8c6b5b557f/zeroize-1.9.0/src/lib.rs', lines 495:8-495:68
+    Name pattern: [zeroize::Zeroize<(@A, @B)>] -/
+@[reducible, rust_trait_impl "zeroize::Zeroize<(@A, @B)>"]
+def Pair.Insts.ZeroizeZeroize {A : Type} {B : Type} (ZeroizeInst :
+  zeroize.Zeroize A) (ZeroizeInst1 : zeroize.Zeroize B) : zeroize.Zeroize (A ×
+  B) := {
+  zeroize := Pair.Insts.ZeroizeZeroize.zeroize ZeroizeInst ZeroizeInst1
 }
 
 /-- [zeroize::{impl zeroize::Zeroize for alloc::vec::Vec<Z>}::zeroize]:
@@ -612,6 +658,52 @@ def Chains.Insts.CoreDefaultDefault : core.default.Default Chains := {
   default := Chains.Insts.CoreDefaultDefault.default
 }
 
+/-- [tacenta_spqr::{impl zeroize::Zeroize for tacenta_spqr::Chains}::zeroize]:
+    Source: 'spqr/src/lib.rs', lines 167:25-167:32
+    Visibility: public -/
+def Chains.Insts.ZeroizeZeroize.zeroize (self : Chains) : Result Chains := do
+  let send ←
+    core.option.Option.Insts.ZeroizeZeroize.zeroize Chain.Insts.ZeroizeZeroize
+      self.send
+  let receive ←
+    core.option.Option.Insts.ZeroizeZeroize.zeroize Chain.Insts.ZeroizeZeroize
+      self.receive
+  ok { send, receive }
+
+/-- Trait implementation: [tacenta_spqr::{impl zeroize::Zeroize for tacenta_spqr::Chains}]
+    Source: 'spqr/src/lib.rs', lines 167:25-167:32 -/
+@[reducible]
+def Chains.Insts.ZeroizeZeroize : zeroize.Zeroize Chains := {
+  zeroize := Chains.Insts.ZeroizeZeroize.zeroize
+}
+
+/-- [tacenta_spqr::{impl core::ops::drop::Drop for tacenta_spqr::Chains}::drop]:
+    Source: 'spqr/src/lib.rs', lines 167:34-167:47
+    Visibility: public -/
+def Chains.Insts.CoreOpsDropDrop.drop (self : Chains) : Result Chains := do
+  let send ←
+    zeroize.__internal.AssertZeroize.Blanket.zeroize_or_on_drop
+      (core.option.Option.Insts.ZeroizeZeroize Chain.Insts.ZeroizeZeroize)
+      self.send
+  let receive ←
+    zeroize.__internal.AssertZeroize.Blanket.zeroize_or_on_drop
+      (core.option.Option.Insts.ZeroizeZeroize Chain.Insts.ZeroizeZeroize)
+      self.receive
+  ok { send, receive }
+
+/-- Trait implementation: [tacenta_spqr::{impl core::ops::drop::Drop for tacenta_spqr::Chains}]
+    Source: 'spqr/src/lib.rs', lines 167:34-167:47 -/
+@[reducible]
+def Chains.Insts.CoreOpsDropDrop : core.ops.drop.Drop Chains := {
+  drop := Chains.Insts.CoreOpsDropDrop.drop
+}
+
+/-- Trait implementation: [tacenta_spqr::{impl zeroize::ZeroizeOnDrop for tacenta_spqr::Chains}]
+    Source: 'spqr/src/lib.rs', lines 167:34-167:47 -/
+@[reducible]
+def Chains.Insts.ZeroizeZeroizeOnDrop : zeroize.ZeroizeOnDrop Chains := {
+}
+
 /-- [tacenta_spqr::Skipped]
     Source: 'spqr/src/lib.rs', lines 177:0-183:1 -/
 structure Skipped where
@@ -705,28 +797,35 @@ def State.Insts.CoreCloneClone : core.clone.Clone State := {
 }
 
 /-- [tacenta_spqr::{impl core::ops::drop::Drop for tacenta_spqr::State}::drop]:
-    Source: 'spqr/src/lib.rs', lines 243:4-245:5
+    Source: 'spqr/src/lib.rs', lines 243:4-247:5
     Visibility: public -/
 def State.Insts.CoreOpsDropDrop.drop (self : State) : Result State := do
   let a ←
     Array.Insts.ZeroizeZeroize.zeroize (zeroize.Zeroize.Blanket
       U8.Insts.ZeroizeDefaultIsZeroes) self.rk
-  ok { self with rk := a }
+  let v ←
+    alloc.vec.Vec.Insts.ZeroizeZeroize.zeroize (Pair.Insts.ZeroizeZeroize
+      (zeroize.Zeroize.Blanket U64.Insts.ZeroizeDefaultIsZeroes)
+      Chains.Insts.ZeroizeZeroize) self.chains
+  let v1 ←
+    alloc.vec.Vec.Insts.ZeroizeZeroize.zeroize Skipped.Insts.ZeroizeZeroize
+      self.skipped
+  ok { self with rk := a, chains := v, skipped := v1 }
 
 /-- Trait implementation: [tacenta_spqr::{impl core::ops::drop::Drop for tacenta_spqr::State}]
-    Source: 'spqr/src/lib.rs', lines 242:0-246:1 -/
+    Source: 'spqr/src/lib.rs', lines 242:0-248:1 -/
 @[reducible]
 def State.Insts.CoreOpsDropDrop : core.ops.drop.Drop State := {
   drop := State.Insts.CoreOpsDropDrop.drop
 }
 
 /-- [tacenta_spqr::be64]:
-    Source: 'spqr/src/lib.rs', lines 262:0-264:1 -/
+    Source: 'spqr/src/lib.rs', lines 264:0-266:1 -/
 def be64 (n : Std.U64) : Result (Array Std.U8 8#usize) := do
   ok (core.num.U64.to_be_bytes n)
 
 /-- [tacenta_spqr::split3]:
-    Source: 'spqr/src/lib.rs', lines 267:0-275:1 -/
+    Source: 'spqr/src/lib.rs', lines 269:0-277:1 -/
 def split3
   (out : Array Std.U8 96#usize) :
   Result ((Array Std.U8 32#usize) × (Array Std.U8 32#usize) × (Array Std.U8
@@ -759,7 +858,7 @@ def split3
   ok (a1, b1, c1)
 
 /-- [tacenta_spqr::info]:
-    Source: 'spqr/src/lib.rs', lines 277:0-282:1 -/
+    Source: 'spqr/src/lib.rs', lines 279:0-284:1 -/
 def info (suffix : Slice Std.U8) : Result (alloc.vec.Vec Std.U8) := do
   let i := Slice.len PROTOCOL_INFO
   let i1 := Slice.len suffix
@@ -769,7 +868,7 @@ def info (suffix : Slice Std.U8) : Result (alloc.vec.Vec Std.U8) := do
   alloc.vec.Vec.extend_from_slice core.clone.CloneU8 v1 suffix
 
 /-- [tacenta_spqr::kdf_init]:
-    Source: 'spqr/src/lib.rs', lines 286:0-295:1 -/
+    Source: 'spqr/src/lib.rs', lines 288:0-297:1 -/
 def kdf_init
   (sk : Slice Std.U8) :
   Result ((Array Std.U8 32#usize) × (Array Std.U8 32#usize) × (Array Std.U8
@@ -789,7 +888,7 @@ def kdf_init
   split3 a2
 
 /-- [tacenta_spqr::kdf_rk]:
-    Source: 'spqr/src/lib.rs', lines 298:0-301:1 -/
+    Source: 'spqr/src/lib.rs', lines 300:0-303:1 -/
 def kdf_rk
   (rk : Array Std.U8 32#usize) (k : Array Std.U8 32#usize) :
   Result ((Array Std.U8 32#usize) × (Array Std.U8 32#usize) × (Array Std.U8
@@ -809,7 +908,7 @@ def kdf_rk
   split3 a1
 
 /-- [tacenta_spqr::kdf_ck]:
-    Source: 'spqr/src/lib.rs', lines 313:0-324:1
+    Source: 'spqr/src/lib.rs', lines 315:0-326:1
     Visibility: public -/
 def kdf_ck
   (ck : Array Std.U8 32#usize) (n : Std.U64) :
@@ -846,7 +945,7 @@ def kdf_ck
   ok (next1, mk1)
 
 /-- [tacenta_spqr::{tacenta_spqr::State}::init]:
-    Source: 'spqr/src/lib.rs', lines 339:4-358:5
+    Source: 'spqr/src/lib.rs', lines 341:4-360:5
     Visibility: public -/
 def State.init (sk : Slice Std.U8) (direction : Direction) : Result State := do
   let (rk, k1, k2) ← kdf_init sk
@@ -874,31 +973,31 @@ def State.init (sk : Slice Std.U8) (direction : Direction) : Result State := do
     }
 
 /-- [tacenta_spqr::{tacenta_spqr::State}::init_alice]:
-    Source: 'spqr/src/lib.rs', lines 328:4-330:5
+    Source: 'spqr/src/lib.rs', lines 330:4-332:5
     Visibility: public -/
 def State.init_alice (sk : Slice Std.U8) : Result State := do
   State.init sk Direction.A2b
 
 /-- [tacenta_spqr::{tacenta_spqr::State}::init_bob]:
-    Source: 'spqr/src/lib.rs', lines 333:4-335:5
+    Source: 'spqr/src/lib.rs', lines 335:4-337:5
     Visibility: public -/
 def State.init_bob (sk : Slice Std.U8) : Result State := do
   State.init sk Direction.B2a
 
 /-- [tacenta_spqr::{tacenta_spqr::State}::epoch]:
-    Source: 'spqr/src/lib.rs', lines 361:4-363:5
+    Source: 'spqr/src/lib.rs', lines 363:4-365:5
     Visibility: public -/
 def State.impl.epoch (self : State) : Result Std.U64 := do
   ok self.epoch
 
 /-- [tacenta_spqr::{tacenta_spqr::State}::skipped_len]:
-    Source: 'spqr/src/lib.rs', lines 367:4-369:5
+    Source: 'spqr/src/lib.rs', lines 369:4-371:5
     Visibility: public -/
 def State.skipped_len (self : State) : Result Std.Usize := do
   ok (alloc.vec.Vec.len self.skipped)
 
 /-- [tacenta_spqr::{tacenta_spqr::State}::find_chains]: loop body 0:
-    Source: 'spqr/src/lib.rs', lines 542:8-549:5 -/
+    Source: 'spqr/src/lib.rs', lines 544:8-551:5 -/
 @[rust_loop_body]
 def State.find_chains_loop.body
   (self : State) (e : Std.U64) (i : Std.Usize) :
@@ -917,7 +1016,7 @@ def State.find_chains_loop.body
   else ok (done none)
 
 /-- [tacenta_spqr::{tacenta_spqr::State}::find_chains]: loop 0:
-    Source: 'spqr/src/lib.rs', lines 542:8-549:5 -/
+    Source: 'spqr/src/lib.rs', lines 544:8-551:5 -/
 @[rust_loop]
 def State.find_chains_loop
   (self : State) (e : Std.U64) (i : Std.Usize) : Result (Option Chains) := do
@@ -926,14 +1025,14 @@ def State.find_chains_loop
     i
 
 /-- [tacenta_spqr::{tacenta_spqr::State}::find_chains]:
-    Source: 'spqr/src/lib.rs', lines 540:4-549:5 -/
+    Source: 'spqr/src/lib.rs', lines 542:4-551:5 -/
 @[reducible]
 def State.find_chains
   (self : State) (e : Std.U64) : Result (Option Chains) := do
   State.find_chains_loop self e 0#usize
 
 /-- [tacenta_spqr::{tacenta_spqr::State}::receive_count]:
-    Source: 'spqr/src/lib.rs', lines 388:4-396:5
+    Source: 'spqr/src/lib.rs', lines 390:4-398:5
     Visibility: public -/
 def State.receive_count
   (self : State) (epoch : Std.U64) : Result (Option Std.U64) := do
@@ -946,13 +1045,13 @@ def State.receive_count
     | some ch => ok (some ch.n)
 
 /-- [tacenta_spqr::{tacenta_spqr::State}::direction]:
-    Source: 'spqr/src/lib.rs', lines 400:4-402:5
+    Source: 'spqr/src/lib.rs', lines 402:4-404:5
     Visibility: public -/
 def State.impl.direction (self : State) : Result Direction := do
   ok self.direction
 
 /-- [tacenta_spqr::{tacenta_spqr::State}::invariant]: loop body 1:
-    Source: 'spqr/src/lib.rs', lines 478:12-483:13
+    Source: 'spqr/src/lib.rs', lines 480:12-485:13
     Visibility: public -/
 @[rust_loop_body]
 def State.invariant_loop0_loop0.body
@@ -974,7 +1073,7 @@ def State.invariant_loop0_loop0.body
   else ok (done chains_ok)
 
 /-- [tacenta_spqr::{tacenta_spqr::State}::invariant]: loop 1:
-    Source: 'spqr/src/lib.rs', lines 478:12-483:13
+    Source: 'spqr/src/lib.rs', lines 480:12-485:13
     Visibility: public -/
 @[rust_loop]
 def State.invariant_loop0_loop0
@@ -988,7 +1087,7 @@ def State.invariant_loop0_loop0
     (chains_ok, j)
 
 /-- [tacenta_spqr::{tacenta_spqr::State}::invariant]: loop body 0:
-    Source: 'spqr/src/lib.rs', lines 469:8-485:9
+    Source: 'spqr/src/lib.rs', lines 471:8-487:9
     Visibility: public -/
 @[rust_loop_body]
 def State.invariant_loop0.body
@@ -1022,7 +1121,7 @@ def State.invariant_loop0.body
   else ok (done (self.chains, self.skipped, chains_ok, current_present))
 
 /-- [tacenta_spqr::{tacenta_spqr::State}::invariant]: loop 0:
-    Source: 'spqr/src/lib.rs', lines 469:8-485:9
+    Source: 'spqr/src/lib.rs', lines 471:8-487:9
     Visibility: public -/
 @[rust_loop]
 def State.invariant_loop0
@@ -1036,7 +1135,7 @@ def State.invariant_loop0
     (chains_ok, current_present, i)
 
 /-- [tacenta_spqr::{tacenta_spqr::State}::invariant]: loop body 3:
-    Source: 'spqr/src/lib.rs', lines 491:12-496:13
+    Source: 'spqr/src/lib.rs', lines 493:12-498:13
     Visibility: public -/
 @[rust_loop_body]
 def State.invariant_loop1_loop0.body
@@ -1060,7 +1159,7 @@ def State.invariant_loop1_loop0.body
   else ok (done present)
 
 /-- [tacenta_spqr::{tacenta_spqr::State}::invariant]: loop 3:
-    Source: 'spqr/src/lib.rs', lines 491:12-496:13
+    Source: 'spqr/src/lib.rs', lines 493:12-498:13
     Visibility: public -/
 @[rust_loop]
 def State.invariant_loop1_loop0
@@ -1073,7 +1172,7 @@ def State.invariant_loop1_loop0
     (present, k)
 
 /-- [tacenta_spqr::{tacenta_spqr::State}::invariant]: loop body 4:
-    Source: 'spqr/src/lib.rs', lines 1:0-508:13
+    Source: 'spqr/src/lib.rs', lines 1:0-510:13
     Visibility: public -/
 @[rust_loop_body]
 def State.invariant_loop1_loop1.body
@@ -1099,7 +1198,7 @@ def State.invariant_loop1_loop1.body
   else ok (done skipped_ok)
 
 /-- [tacenta_spqr::{tacenta_spqr::State}::invariant]: loop 4:
-    Source: 'spqr/src/lib.rs', lines 1:0-508:13
+    Source: 'spqr/src/lib.rs', lines 1:0-510:13
     Visibility: public -/
 @[rust_loop]
 def State.invariant_loop1_loop1
@@ -1113,7 +1212,7 @@ def State.invariant_loop1_loop1
     (skipped_ok, j)
 
 /-- [tacenta_spqr::{tacenta_spqr::State}::invariant]: loop body 2:
-    Source: 'spqr/src/lib.rs', lines 1:0-510:9
+    Source: 'spqr/src/lib.rs', lines 1:0-512:9
     Visibility: public -/
 @[rust_loop_body]
 def State.invariant_loop1.body
@@ -1135,7 +1234,7 @@ def State.invariant_loop1.body
   else ok (done skipped_ok)
 
 /-- [tacenta_spqr::{tacenta_spqr::State}::invariant]: loop 2:
-    Source: 'spqr/src/lib.rs', lines 1:0-510:9
+    Source: 'spqr/src/lib.rs', lines 1:0-512:9
     Visibility: public -/
 @[rust_loop]
 def State.invariant_loop1
@@ -1148,7 +1247,7 @@ def State.invariant_loop1
     (skipped_ok, i)
 
 /-- [tacenta_spqr::{tacenta_spqr::State}::invariant]:
-    Source: 'spqr/src/lib.rs', lines 465:4-512:5
+    Source: 'spqr/src/lib.rs', lines 467:4-514:5
     Visibility: public -/
 def State.invariant (self : State) : Result Bool := do
   let (v, v1, chains_ok, current_present) ←
@@ -1165,7 +1264,7 @@ def State.invariant (self : State) : Result Bool := do
   else ok false
 
 /-- [tacenta_spqr::{tacenta_spqr::State}::evict_oldest]: loop body 0:
-    Source: 'spqr/src/lib.rs', lines 1:0-536:9
+    Source: 'spqr/src/lib.rs', lines 1:0-538:9
     Visibility: public -/
 @[rust_loop_body]
 def State.evict_oldest_loop.body
@@ -1184,7 +1283,7 @@ def State.evict_oldest_loop.body
   else ok (done (evicted, self))
 
 /-- [tacenta_spqr::{tacenta_spqr::State}::evict_oldest]: loop 0:
-    Source: 'spqr/src/lib.rs', lines 1:0-536:9
+    Source: 'spqr/src/lib.rs', lines 1:0-538:9
     Visibility: public -/
 @[rust_loop]
 def State.evict_oldest_loop
@@ -1197,7 +1296,7 @@ def State.evict_oldest_loop
     (self, evicted)
 
 /-- [tacenta_spqr::{tacenta_spqr::State}::evict_oldest]:
-    Source: 'spqr/src/lib.rs', lines 531:4-538:5
+    Source: 'spqr/src/lib.rs', lines 533:4-540:5
     Visibility: public -/
 @[reducible]
 def State.evict_oldest
@@ -1205,12 +1304,12 @@ def State.evict_oldest
   State.evict_oldest_loop self count 0#usize
 
 /-- [tacenta_spqr::{tacenta_spqr::State}::set_chains::closure]
-    Source: 'spqr/src/lib.rs', lines 552:27-552:39 -/
+    Source: 'spqr/src/lib.rs', lines 554:27-554:39 -/
 @[reducible]
 def State.set_chains.closure := Std.U64
 
 /-- [tacenta_spqr::{tacenta_spqr::State}::set_chains::{impl core::ops::function::FnMut<(&'_ (u64, tacenta_spqr::Chains),), bool> for tacenta_spqr::{tacenta_spqr::State}::set_chains::closure<'_0>}::call_mut]:
-    Source: 'spqr/src/lib.rs', lines 552:27-552:39 -/
+    Source: 'spqr/src/lib.rs', lines 554:27-554:39 -/
 def
   State.set_chains.closure.Insts.CoreOpsFunctionFnMutTupleSharedPairU64ChainsBool.call_mut
   (c : State.set_chains.closure) (tupled_args : (Std.U64 × Chains)) :
@@ -1220,7 +1319,7 @@ def
   ok (i != c, c)
 
 /-- [tacenta_spqr::{tacenta_spqr::State}::set_chains::{impl core::ops::function::FnOnce<(&'_ (u64, tacenta_spqr::Chains),), bool> for tacenta_spqr::{tacenta_spqr::State}::set_chains::closure<'_0>}::call_once]:
-    Source: 'spqr/src/lib.rs', lines 552:27-552:39 -/
+    Source: 'spqr/src/lib.rs', lines 554:27-554:39 -/
 def
   State.set_chains.closure.Insts.CoreOpsFunctionFnOnceTupleSharedPairU64ChainsBool.call_once
   (c : State.set_chains.closure) (p : (Std.U64 × Chains)) : Result Bool := do
@@ -1230,7 +1329,7 @@ def
   ok b
 
 /-- Trait implementation: [tacenta_spqr::{tacenta_spqr::State}::set_chains::{impl core::ops::function::FnOnce<(&'_ (u64, tacenta_spqr::Chains),), bool> for tacenta_spqr::{tacenta_spqr::State}::set_chains::closure<'_0>}]
-    Source: 'spqr/src/lib.rs', lines 552:27-552:39 -/
+    Source: 'spqr/src/lib.rs', lines 554:27-554:39 -/
 @[reducible]
 def
   State.set_chains.closure.Insts.CoreOpsFunctionFnOnceTupleSharedPairU64ChainsBool
@@ -1241,7 +1340,7 @@ def
 }
 
 /-- Trait implementation: [tacenta_spqr::{tacenta_spqr::State}::set_chains::{impl core::ops::function::FnMut<(&'_ (u64, tacenta_spqr::Chains),), bool> for tacenta_spqr::{tacenta_spqr::State}::set_chains::closure<'_0>}]
-    Source: 'spqr/src/lib.rs', lines 552:27-552:39 -/
+    Source: 'spqr/src/lib.rs', lines 554:27-554:39 -/
 @[reducible]
 def
   State.set_chains.closure.Insts.CoreOpsFunctionFnMutTupleSharedPairU64ChainsBool
@@ -1254,7 +1353,7 @@ def
 }
 
 /-- [tacenta_spqr::{tacenta_spqr::State}::set_chains]:
-    Source: 'spqr/src/lib.rs', lines 551:4-554:5 -/
+    Source: 'spqr/src/lib.rs', lines 553:4-556:5 -/
 def State.set_chains
   (self : State) (e : Std.U64) (c : Chains) : Result State := do
   let v ←
@@ -1265,12 +1364,12 @@ def State.set_chains
   ok { self with chains := v1 }
 
 /-- [tacenta_spqr::{tacenta_spqr::State}::clear_old_epochs::closure#1]
-    Source: 'spqr/src/lib.rs', lines 562:20-562:69 -/
+    Source: 'spqr/src/lib.rs', lines 564:20-564:69 -/
 @[reducible]
 def State.clear_old_epochs.closure_1 := Std.U64
 
 /-- [tacenta_spqr::{tacenta_spqr::State}::clear_old_epochs::{impl core::ops::function::FnMut<(&'_ tacenta_spqr::Skipped,), bool> for tacenta_spqr::{tacenta_spqr::State}::clear_old_epochs::closure#1<'_0>}::call_mut]:
-    Source: 'spqr/src/lib.rs', lines 562:20-562:69 -/
+    Source: 'spqr/src/lib.rs', lines 564:20-564:69 -/
 def
   State.clear_old_epochs.closure_1.Insts.CoreOpsFunctionFnMutTupleSharedSkippedBool.call_mut
   (c : State.clear_old_epochs.closure_1) (tupled_args : Skipped) :
@@ -1280,7 +1379,7 @@ def
   ok (c < i, c)
 
 /-- [tacenta_spqr::{tacenta_spqr::State}::clear_old_epochs::{impl core::ops::function::FnOnce<(&'_ tacenta_spqr::Skipped,), bool> for tacenta_spqr::{tacenta_spqr::State}::clear_old_epochs::closure#1<'_0>}::call_once]:
-    Source: 'spqr/src/lib.rs', lines 562:20-562:69 -/
+    Source: 'spqr/src/lib.rs', lines 564:20-564:69 -/
 def
   State.clear_old_epochs.closure_1.Insts.CoreOpsFunctionFnOnceTupleSharedSkippedBool.call_once
   (c : State.clear_old_epochs.closure_1) (s : Skipped) : Result Bool := do
@@ -1290,7 +1389,7 @@ def
   ok b
 
 /-- Trait implementation: [tacenta_spqr::{tacenta_spqr::State}::clear_old_epochs::{impl core::ops::function::FnOnce<(&'_ tacenta_spqr::Skipped,), bool> for tacenta_spqr::{tacenta_spqr::State}::clear_old_epochs::closure#1<'_0>}]
-    Source: 'spqr/src/lib.rs', lines 562:20-562:69 -/
+    Source: 'spqr/src/lib.rs', lines 564:20-564:69 -/
 @[reducible]
 def
   State.clear_old_epochs.closure_1.Insts.CoreOpsFunctionFnOnceTupleSharedSkippedBool
@@ -1300,7 +1399,7 @@ def
 }
 
 /-- Trait implementation: [tacenta_spqr::{tacenta_spqr::State}::clear_old_epochs::{impl core::ops::function::FnMut<(&'_ tacenta_spqr::Skipped,), bool> for tacenta_spqr::{tacenta_spqr::State}::clear_old_epochs::closure#1<'_0>}]
-    Source: 'spqr/src/lib.rs', lines 562:20-562:69 -/
+    Source: 'spqr/src/lib.rs', lines 564:20-564:69 -/
 @[reducible]
 def
   State.clear_old_epochs.closure_1.Insts.CoreOpsFunctionFnMutTupleSharedSkippedBool
@@ -1312,12 +1411,12 @@ def
 }
 
 /-- [tacenta_spqr::{tacenta_spqr::State}::clear_old_epochs::closure]
-    Source: 'spqr/src/lib.rs', lines 560:20-560:65 -/
+    Source: 'spqr/src/lib.rs', lines 562:20-562:65 -/
 @[reducible]
 def State.clear_old_epochs.closure := Std.U64
 
 /-- [tacenta_spqr::{tacenta_spqr::State}::clear_old_epochs::{impl core::ops::function::FnMut<(&'_ (u64, tacenta_spqr::Chains),), bool> for tacenta_spqr::{tacenta_spqr::State}::clear_old_epochs::closure<'_0>}::call_mut]:
-    Source: 'spqr/src/lib.rs', lines 560:20-560:65 -/
+    Source: 'spqr/src/lib.rs', lines 562:20-562:65 -/
 def
   State.clear_old_epochs.closure.Insts.CoreOpsFunctionFnMutTupleSharedPairU64ChainsBool.call_mut
   (c : State.clear_old_epochs.closure) (tupled_args : (Std.U64 × Chains)) :
@@ -1328,7 +1427,7 @@ def
   ok (c < i1, c)
 
 /-- [tacenta_spqr::{tacenta_spqr::State}::clear_old_epochs::{impl core::ops::function::FnOnce<(&'_ (u64, tacenta_spqr::Chains),), bool> for tacenta_spqr::{tacenta_spqr::State}::clear_old_epochs::closure<'_0>}::call_once]:
-    Source: 'spqr/src/lib.rs', lines 560:20-560:65 -/
+    Source: 'spqr/src/lib.rs', lines 562:20-562:65 -/
 def
   State.clear_old_epochs.closure.Insts.CoreOpsFunctionFnOnceTupleSharedPairU64ChainsBool.call_once
   (c : State.clear_old_epochs.closure) (p : (Std.U64 × Chains)) :
@@ -1340,7 +1439,7 @@ def
   ok b
 
 /-- Trait implementation: [tacenta_spqr::{tacenta_spqr::State}::clear_old_epochs::{impl core::ops::function::FnOnce<(&'_ (u64, tacenta_spqr::Chains),), bool> for tacenta_spqr::{tacenta_spqr::State}::clear_old_epochs::closure<'_0>}]
-    Source: 'spqr/src/lib.rs', lines 560:20-560:65 -/
+    Source: 'spqr/src/lib.rs', lines 562:20-562:65 -/
 @[reducible]
 def
   State.clear_old_epochs.closure.Insts.CoreOpsFunctionFnOnceTupleSharedPairU64ChainsBool
@@ -1351,7 +1450,7 @@ def
 }
 
 /-- Trait implementation: [tacenta_spqr::{tacenta_spqr::State}::clear_old_epochs::{impl core::ops::function::FnMut<(&'_ (u64, tacenta_spqr::Chains),), bool> for tacenta_spqr::{tacenta_spqr::State}::clear_old_epochs::closure<'_0>}]
-    Source: 'spqr/src/lib.rs', lines 560:20-560:65 -/
+    Source: 'spqr/src/lib.rs', lines 562:20-562:65 -/
 @[reducible]
 def
   State.clear_old_epochs.closure.Insts.CoreOpsFunctionFnMutTupleSharedPairU64ChainsBool
@@ -1364,7 +1463,7 @@ def
 }
 
 /-- [tacenta_spqr::{tacenta_spqr::State}::clear_old_epochs]:
-    Source: 'spqr/src/lib.rs', lines 558:4-563:5 -/
+    Source: 'spqr/src/lib.rs', lines 560:4-565:5 -/
 def State.clear_old_epochs
   (self : State) (current : Std.U64) : Result State := do
   let v ←
@@ -1378,7 +1477,7 @@ def State.clear_old_epochs
   ok { self with chains := v, skipped := v1 }
 
 /-- [tacenta_spqr::{tacenta_spqr::State}::advance]:
-    Source: 'spqr/src/lib.rs', lines 580:4-607:5 -/
+    Source: 'spqr/src/lib.rs', lines 582:4-609:5 -/
 def State.advance
   (self : State) (out : Output) :
   Result ((core.result.Result Unit SpqrError) × State)
@@ -1413,7 +1512,7 @@ def State.advance
         ok (core.result.Result.Ok (), self2)
 
 /-- [tacenta_spqr::{tacenta_spqr::State}::maybe_advance]:
-    Source: 'spqr/src/lib.rs', lines 609:4-614:5 -/
+    Source: 'spqr/src/lib.rs', lines 611:4-616:5 -/
 def State.maybe_advance
   (self : State) (out : Option Output) :
   Result ((core.result.Result Unit SpqrError) × State)
@@ -1423,7 +1522,7 @@ def State.maybe_advance
   | some o => State.advance self o
 
 /-- [tacenta_spqr::{tacenta_spqr::State}::send]:
-    Source: 'spqr/src/lib.rs', lines 622:4-648:5
+    Source: 'spqr/src/lib.rs', lines 624:4-650:5
     Visibility: public -/
 def State.send
   (self : State) (sending_epoch : Std.U64) (out : Option Output) :
@@ -1463,7 +1562,7 @@ def State.send
     ok (r1, self1)
 
 /-- [tacenta_spqr::{tacenta_spqr::State}::try_skipped]: loop body 0:
-    Source: 'spqr/src/lib.rs', lines 1:0-662:5 -/
+    Source: 'spqr/src/lib.rs', lines 1:0-664:5 -/
 @[rust_loop_body]
 def State.try_skipped_loop.body
   (self : State) (e : Std.U64) (n : Std.U64) (i : Std.Usize) :
@@ -1493,7 +1592,7 @@ def State.try_skipped_loop.body
       self.direction))
 
 /-- [tacenta_spqr::{tacenta_spqr::State}::try_skipped]: loop 0:
-    Source: 'spqr/src/lib.rs', lines 1:0-662:5 -/
+    Source: 'spqr/src/lib.rs', lines 1:0-664:5 -/
 @[rust_loop]
 def State.try_skipped_loop
   (self : State) (e : Std.U64) (n : Std.U64) (i : Std.Usize) :
@@ -1506,7 +1605,7 @@ def State.try_skipped_loop
     i
 
 /-- [tacenta_spqr::{tacenta_spqr::State}::try_skipped]:
-    Source: 'spqr/src/lib.rs', lines 652:4-662:5 -/
+    Source: 'spqr/src/lib.rs', lines 654:4-664:5 -/
 def State.try_skipped
   (self : State) (e : Std.U64) (n : Std.U64) :
   Result ((Option (Array Std.U8 32#usize)) × State)
@@ -1515,11 +1614,11 @@ def State.try_skipped
   ok (o, { rk := a, epoch := i, chains := v, skipped := v1, direction := d })
 
 /-- [tacenta_spqr::{tacenta_spqr::State}::skip_message_keys::closure]
-    Source: 'spqr/src/lib.rs', lines 707:20-707:68 -/
+    Source: 'spqr/src/lib.rs', lines 709:20-709:68 -/
 def State.skip_message_keys.closure := Std.U64 × Std.U64 × Std.U64
 
 /-- [tacenta_spqr::{tacenta_spqr::State}::skip_message_keys::{impl core::ops::function::FnMut<(&'_ tacenta_spqr::Skipped,), bool> for tacenta_spqr::{tacenta_spqr::State}::skip_message_keys::closure<'_0, '_1, '_2>}::call_mut]:
-    Source: 'spqr/src/lib.rs', lines 707:20-707:68 -/
+    Source: 'spqr/src/lib.rs', lines 709:20-709:68 -/
 def
   State.skip_message_keys.closure.Insts.CoreOpsFunctionFnMutTupleSharedSkippedBool.call_mut
   (c : State.skip_message_keys.closure) (tupled_args : Skipped) :
@@ -1535,7 +1634,7 @@ def
   ok (¬ b, c)
 
 /-- [tacenta_spqr::{tacenta_spqr::State}::skip_message_keys::{impl core::ops::function::FnOnce<(&'_ tacenta_spqr::Skipped,), bool> for tacenta_spqr::{tacenta_spqr::State}::skip_message_keys::closure<'_0, '_1, '_2>}::call_once]:
-    Source: 'spqr/src/lib.rs', lines 707:20-707:68 -/
+    Source: 'spqr/src/lib.rs', lines 709:20-709:68 -/
 def
   State.skip_message_keys.closure.Insts.CoreOpsFunctionFnOnceTupleSharedSkippedBool.call_once
   (c : State.skip_message_keys.closure) (s : Skipped) : Result Bool := do
@@ -1545,7 +1644,7 @@ def
   ok b
 
 /-- Trait implementation: [tacenta_spqr::{tacenta_spqr::State}::skip_message_keys::{impl core::ops::function::FnOnce<(&'_ tacenta_spqr::Skipped,), bool> for tacenta_spqr::{tacenta_spqr::State}::skip_message_keys::closure<'_0, '_1, '_2>}]
-    Source: 'spqr/src/lib.rs', lines 707:20-707:68 -/
+    Source: 'spqr/src/lib.rs', lines 709:20-709:68 -/
 @[reducible]
 def
   State.skip_message_keys.closure.Insts.CoreOpsFunctionFnOnceTupleSharedSkippedBool
@@ -1555,7 +1654,7 @@ def
 }
 
 /-- Trait implementation: [tacenta_spqr::{tacenta_spqr::State}::skip_message_keys::{impl core::ops::function::FnMut<(&'_ tacenta_spqr::Skipped,), bool> for tacenta_spqr::{tacenta_spqr::State}::skip_message_keys::closure<'_0, '_1, '_2>}]
-    Source: 'spqr/src/lib.rs', lines 707:20-707:68 -/
+    Source: 'spqr/src/lib.rs', lines 709:20-709:68 -/
 @[reducible]
 def
   State.skip_message_keys.closure.Insts.CoreOpsFunctionFnMutTupleSharedSkippedBool
@@ -1567,7 +1666,7 @@ def
 }
 
 /-- [tacenta_spqr::{tacenta_spqr::State}::skip_message_keys]: loop body 0:
-    Source: 'spqr/src/lib.rs', lines 694:8-704:9 -/
+    Source: 'spqr/src/lib.rs', lines 696:8-706:9 -/
 @[rust_loop_body]
 def State.skip_message_keys_loop.body
   (e : Std.U64) (upto : Std.U64) (ck : Array Std.U8 32#usize)
@@ -1589,7 +1688,7 @@ def State.skip_message_keys_loop.body
   else ok (done (ck, derived))
 
 /-- [tacenta_spqr::{tacenta_spqr::State}::skip_message_keys]: loop 0:
-    Source: 'spqr/src/lib.rs', lines 694:8-704:9 -/
+    Source: 'spqr/src/lib.rs', lines 696:8-706:9 -/
 @[rust_loop]
 def State.skip_message_keys_loop
   (e : Std.U64) (upto : Std.U64) (ck : Array Std.U8 32#usize)
@@ -1602,7 +1701,7 @@ def State.skip_message_keys_loop
     (ck, derived, num)
 
 /-- [tacenta_spqr::{tacenta_spqr::State}::skip_message_keys]:
-    Source: 'spqr/src/lib.rs', lines 669:4-717:5 -/
+    Source: 'spqr/src/lib.rs', lines 671:4-719:5 -/
 def State.skip_message_keys
   (self : State) (e : Std.U64) (upto : Std.U64) :
   Result ((core.result.Result Unit SpqrError) × State)
@@ -1647,7 +1746,7 @@ def State.skip_message_keys
             ok (core.result.Result.Ok (), self1)
 
 /-- [tacenta_spqr::{tacenta_spqr::State}::receive]:
-    Source: 'spqr/src/lib.rs', lines 731:4-769:5
+    Source: 'spqr/src/lib.rs', lines 733:4-771:5
     Visibility: public -/
 def State.receive
   (self : State) (receiving_epoch : Std.U64) (out : Option Output)
@@ -1704,11 +1803,11 @@ def State.receive
     ok (r1, self1)
 
 /-- [tacenta_spqr::STATE_VERSION]
-    Source: 'spqr/src/lib.rs', lines 776:0-776:31 -/
+    Source: 'spqr/src/lib.rs', lines 778:0-778:31 -/
 @[global_simps, irreducible] def STATE_VERSION : Std.U8 := 1#u8
 
 /-- [tacenta_spqr::SpqrDecodeError]
-    Source: 'spqr/src/lib.rs', lines 787:0-791:1
+    Source: 'spqr/src/lib.rs', lines 789:0-793:1
     Visibility: public -/
 @[discriminant isize]
 inductive SpqrDecodeError where
@@ -1717,14 +1816,14 @@ inductive SpqrDecodeError where
 | Malformed : SpqrDecodeError
 
 /-- [tacenta_spqr::{impl core::clone::Clone for tacenta_spqr::SpqrDecodeError}::clone]:
-    Source: 'spqr/src/lib.rs', lines 786:9-786:14
+    Source: 'spqr/src/lib.rs', lines 788:9-788:14
     Visibility: public -/
 def SpqrDecodeError.Insts.CoreCloneClone.clone
   (self : SpqrDecodeError) : Result SpqrDecodeError := do
   ok self
 
 /-- Trait implementation: [tacenta_spqr::{impl core::clone::Clone for tacenta_spqr::SpqrDecodeError}]
-    Source: 'spqr/src/lib.rs', lines 786:9-786:14 -/
+    Source: 'spqr/src/lib.rs', lines 788:9-788:14 -/
 @[reducible]
 def SpqrDecodeError.Insts.CoreCloneClone : core.clone.Clone SpqrDecodeError
   := {
@@ -1732,7 +1831,7 @@ def SpqrDecodeError.Insts.CoreCloneClone : core.clone.Clone SpqrDecodeError
 }
 
 /-- Trait implementation: [tacenta_spqr::{impl core::marker::Copy for tacenta_spqr::SpqrDecodeError}]
-    Source: 'spqr/src/lib.rs', lines 786:16-786:20 -/
+    Source: 'spqr/src/lib.rs', lines 788:16-788:20 -/
 @[reducible]
 def SpqrDecodeError.Insts.CoreMarkerCopy : core.marker.Copy SpqrDecodeError
   := {
@@ -1740,14 +1839,14 @@ def SpqrDecodeError.Insts.CoreMarkerCopy : core.marker.Copy SpqrDecodeError
 }
 
 /-- Trait implementation: [tacenta_spqr::{impl core::marker::StructuralPartialEq for tacenta_spqr::SpqrDecodeError}]
-    Source: 'spqr/src/lib.rs', lines 786:22-786:31 -/
+    Source: 'spqr/src/lib.rs', lines 788:22-788:31 -/
 @[reducible]
 def SpqrDecodeError.Insts.CoreMarkerStructuralPartialEq :
   core.marker.StructuralPartialEq SpqrDecodeError := {
 }
 
 /-- [tacenta_spqr::{impl core::cmp::PartialEq<tacenta_spqr::SpqrDecodeError> for tacenta_spqr::SpqrDecodeError}::eq]:
-    Source: 'spqr/src/lib.rs', lines 786:22-786:31
+    Source: 'spqr/src/lib.rs', lines 788:22-788:31
     Visibility: public -/
 def SpqrDecodeError.Insts.CoreCmpPartialEqSpqrDecodeError.eq
   (self : SpqrDecodeError) (other : SpqrDecodeError) : Result Bool := do
@@ -1756,7 +1855,7 @@ def SpqrDecodeError.Insts.CoreCmpPartialEqSpqrDecodeError.eq
   ok (self1 = other1)
 
 /-- Trait implementation: [tacenta_spqr::{impl core::cmp::PartialEq<tacenta_spqr::SpqrDecodeError> for tacenta_spqr::SpqrDecodeError}]
-    Source: 'spqr/src/lib.rs', lines 786:22-786:31 -/
+    Source: 'spqr/src/lib.rs', lines 788:22-788:31 -/
 @[reducible]
 def SpqrDecodeError.Insts.CoreCmpPartialEqSpqrDecodeError : core.cmp.PartialEq
   SpqrDecodeError SpqrDecodeError := {
@@ -1764,14 +1863,14 @@ def SpqrDecodeError.Insts.CoreCmpPartialEqSpqrDecodeError : core.cmp.PartialEq
 }
 
 /-- [tacenta_spqr::{impl core::cmp::Eq for tacenta_spqr::SpqrDecodeError}::assert_fields_are_eq]:
-    Source: 'spqr/src/lib.rs', lines 786:33-786:35
+    Source: 'spqr/src/lib.rs', lines 788:33-788:35
     Visibility: public -/
 def SpqrDecodeError.Insts.CoreCmpEq.assert_fields_are_eq
   (self : SpqrDecodeError) : Result Unit := do
   ok ()
 
 /-- Trait implementation: [tacenta_spqr::{impl core::cmp::Eq for tacenta_spqr::SpqrDecodeError}]
-    Source: 'spqr/src/lib.rs', lines 786:33-786:35 -/
+    Source: 'spqr/src/lib.rs', lines 788:33-788:35 -/
 @[reducible]
 def SpqrDecodeError.Insts.CoreCmpEq : core.cmp.Eq SpqrDecodeError := {
   partialEqInst := SpqrDecodeError.Insts.CoreCmpPartialEqSpqrDecodeError
@@ -1779,7 +1878,7 @@ def SpqrDecodeError.Insts.CoreCmpEq : core.cmp.Eq SpqrDecodeError := {
 }
 
 /-- [tacenta_spqr::{impl core::fmt::Debug for tacenta_spqr::SpqrDecodeError}::fmt]:
-    Source: 'spqr/src/lib.rs', lines 786:37-786:42
+    Source: 'spqr/src/lib.rs', lines 788:37-788:42
     Visibility: public -/
 def SpqrDecodeError.Insts.CoreFmtDebug.fmt
   (self : SpqrDecodeError) (f : core.fmt.Formatter) :
@@ -1794,20 +1893,20 @@ def SpqrDecodeError.Insts.CoreFmtDebug.fmt
     core.fmt.Formatter.write_str f (toStr "Malformed")
 
 /-- Trait implementation: [tacenta_spqr::{impl core::fmt::Debug for tacenta_spqr::SpqrDecodeError}]
-    Source: 'spqr/src/lib.rs', lines 786:37-786:42 -/
+    Source: 'spqr/src/lib.rs', lines 788:37-788:42 -/
 @[reducible]
 def SpqrDecodeError.Insts.CoreFmtDebug : core.fmt.Debug SpqrDecodeError := {
   fmt := SpqrDecodeError.Insts.CoreFmtDebug.fmt
 }
 
 /-- [tacenta_spqr::CHAIN_LEN]
-    Source: 'spqr/src/lib.rs', lines 796:0-796:36 -/
+    Source: 'spqr/src/lib.rs', lines 798:0-798:36 -/
 @[global_simps, irreducible]
 def CHAIN_LEN : Result Std.Usize := do let i ← 1#usize + 32#usize
                                        i + 8#usize
 
 /-- [tacenta_spqr::CHAINS_LEN]
-    Source: 'spqr/src/lib.rs', lines 797:0-797:44 -/
+    Source: 'spqr/src/lib.rs', lines 799:0-799:44 -/
 @[global_simps, irreducible]
 def CHAINS_LEN : Result Std.Usize := do
   let i ← CHAIN_LEN
@@ -1815,14 +1914,14 @@ def CHAINS_LEN : Result Std.Usize := do
   8#usize + i1
 
 /-- [tacenta_spqr::SKIPPED_LEN]
-    Source: 'spqr/src/lib.rs', lines 798:0-798:38 -/
+    Source: 'spqr/src/lib.rs', lines 800:0-800:38 -/
 @[global_simps, irreducible]
 def SKIPPED_LEN : Result Std.Usize := do
   let i ← 8#usize + 8#usize
   i + 32#usize
 
 /-- [tacenta_spqr::FIXED_PREFIX]
-    Source: 'spqr/src/lib.rs', lines 800:0-804:8 -/
+    Source: 'spqr/src/lib.rs', lines 802:0-806:8 -/
 @[global_simps, irreducible]
 def FIXED_PREFIX : Result Std.Usize := do
   let i ← 1#usize + 32#usize
@@ -1831,14 +1930,14 @@ def FIXED_PREFIX : Result Std.Usize := do
   i2 + 4#usize
 
 /-- [tacenta_spqr::{tacenta_spqr::Direction}::to_byte]:
-    Source: 'spqr/src/lib.rs', lines 807:4-812:5 -/
+    Source: 'spqr/src/lib.rs', lines 809:4-814:5 -/
 def Direction.to_byte (self : Direction) : Result Std.U8 := do
   match self with
   | Direction.A2b => ok 0#u8
   | Direction.B2a => ok 1#u8
 
 /-- [tacenta_spqr::{tacenta_spqr::Direction}::from_byte]:
-    Source: 'spqr/src/lib.rs', lines 814:4-820:5 -/
+    Source: 'spqr/src/lib.rs', lines 816:4-822:5 -/
 def Direction.from_byte (b : Std.U8) : Result (Option Direction) := do
   match b with
   | 0#uscalar => ok (some Direction.A2b)
@@ -1846,7 +1945,7 @@ def Direction.from_byte (b : Std.U8) : Result (Option Direction) := do
   | _ => ok none
 
 /-- [tacenta_spqr::push_optional_chain]:
-    Source: 'spqr/src/lib.rs', lines 823:0-836:1 -/
+    Source: 'spqr/src/lib.rs', lines 825:0-838:1 -/
 def push_optional_chain
   (out : alloc.vec.Vec Std.U8) (chain : Option Chain) :
   Result (alloc.vec.Vec Std.U8)
@@ -1869,7 +1968,7 @@ def push_optional_chain
     alloc.vec.Vec.extend_from_slice core.clone.CloneU8 out2 s1
 
 /-- [tacenta_spqr::decode_chain]: loop body 0:
-    Source: 'spqr/src/lib.rs', lines 858:12-863:13 -/
+    Source: 'spqr/src/lib.rs', lines 860:12-865:13 -/
 @[rust_loop_body]
 def decode_chain_loop.body
   (i : Std.Usize) (bytes : Slice Std.U8) (pos : Std.Usize) (clean : Bool)
@@ -1888,7 +1987,7 @@ def decode_chain_loop.body
   else ok (done clean)
 
 /-- [tacenta_spqr::decode_chain]: loop 0:
-    Source: 'spqr/src/lib.rs', lines 858:12-863:13 -/
+    Source: 'spqr/src/lib.rs', lines 860:12-865:13 -/
 @[rust_loop]
 def decode_chain_loop
   (i : Std.Usize) (bytes : Slice Std.U8) (pos : Std.Usize) (clean : Bool)
@@ -1900,7 +1999,7 @@ def decode_chain_loop
     (clean, i1)
 
 /-- [tacenta_spqr::decode_chain]:
-    Source: 'spqr/src/lib.rs', lines 841:0-878:1 -/
+    Source: 'spqr/src/lib.rs', lines 843:0-880:1 -/
 def decode_chain
   (bytes : Slice Std.U8) (pos : Std.Usize) :
   Result (Option (Option Chain))
@@ -1944,7 +2043,7 @@ def decode_chain
     | _ => ok none
 
 /-- [tacenta_spqr::decode_chains_entry]:
-    Source: 'spqr/src/lib.rs', lines 882:0-897:1 -/
+    Source: 'spqr/src/lib.rs', lines 884:0-899:1 -/
 def decode_chains_entry
   (bytes : Slice Std.U8) (pos : Std.Usize) :
   Result (Option (Std.U64 × Chains))
@@ -1975,7 +2074,7 @@ def decode_chains_entry
         ok (some (i4, { send := v, receive := v1 }))
 
 /-- [tacenta_spqr::decode_skipped_entry]:
-    Source: 'spqr/src/lib.rs', lines 900:0-915:1 -/
+    Source: 'spqr/src/lib.rs', lines 902:0-917:1 -/
 def decode_skipped_entry
   (bytes : Slice Std.U8) (pos : Std.Usize) : Result (Option Skipped) := do
   let i := Slice.len bytes
@@ -2013,7 +2112,7 @@ def decode_skipped_entry
     ok (some { epoch := i6, n := i7, key := key1 })
 
 /-- [tacenta_spqr::{tacenta_spqr::State}::encoded_len]:
-    Source: 'spqr/src/lib.rs', lines 963:4-967:5 -/
+    Source: 'spqr/src/lib.rs', lines 965:4-969:5 -/
 def State.encoded_len (self : State) : Result Std.Usize := do
   let i := alloc.vec.Vec.len self.chains
   let i1 ← CHAINS_LEN
@@ -2027,7 +2126,7 @@ def State.encoded_len (self : State) : Result Std.Usize := do
   i5 + i8
 
 /-- [tacenta_spqr::{tacenta_spqr::State}::to_bytes]: loop body 0:
-    Source: 'spqr/src/lib.rs', lines 931:8-937:9
+    Source: 'spqr/src/lib.rs', lines 933:8-939:9
     Visibility: public -/
 @[rust_loop_body]
 def State.to_bytes_loop0.body
@@ -2052,7 +2151,7 @@ def State.to_bytes_loop0.body
   else ok (done out)
 
 /-- [tacenta_spqr::{tacenta_spqr::State}::to_bytes]: loop 0:
-    Source: 'spqr/src/lib.rs', lines 931:8-937:9
+    Source: 'spqr/src/lib.rs', lines 933:8-939:9
     Visibility: public -/
 @[rust_loop]
 def State.to_bytes_loop0
@@ -2065,7 +2164,7 @@ def State.to_bytes_loop0
     (out, i)
 
 /-- [tacenta_spqr::{tacenta_spqr::State}::to_bytes]: loop body 1:
-    Source: 'spqr/src/lib.rs', lines 940:8-946:9
+    Source: 'spqr/src/lib.rs', lines 942:8-948:9
     Visibility: public -/
 @[rust_loop_body]
 def State.to_bytes_loop1.body
@@ -2091,7 +2190,7 @@ def State.to_bytes_loop1.body
   else ok (done out)
 
 /-- [tacenta_spqr::{tacenta_spqr::State}::to_bytes]: loop 1:
-    Source: 'spqr/src/lib.rs', lines 940:8-946:9
+    Source: 'spqr/src/lib.rs', lines 942:8-948:9
     Visibility: public -/
 @[rust_loop]
 def State.to_bytes_loop1
@@ -2103,7 +2202,7 @@ def State.to_bytes_loop1
     (out, j)
 
 /-- [tacenta_spqr::{tacenta_spqr::State}::to_bytes]:
-    Source: 'spqr/src/lib.rs', lines 922:4-955:5
+    Source: 'spqr/src/lib.rs', lines 924:4-957:5
     Visibility: public -/
 def State.to_bytes
   (self : State) : Result (zeroize.Zeroizing (alloc.vec.Vec Std.U8)) := do
@@ -2135,7 +2234,7 @@ def State.to_bytes
     (zeroize.Zeroize.Blanket U8.Insts.ZeroizeDefaultIsZeroes)) out8
 
 /-- [tacenta_spqr::{tacenta_spqr::State}::from_bytes]: loop body 0:
-    Source: 'spqr/src/lib.rs', lines 1013:8-1021:9
+    Source: 'spqr/src/lib.rs', lines 1015:8-1023:9
     Visibility: public -/
 @[rust_loop_body]
 def State.from_bytes_loop0.body
@@ -2160,7 +2259,7 @@ def State.from_bytes_loop0.body
       ok (cont (iter1, pos1, chains1, chains_ok))
 
 /-- [tacenta_spqr::{tacenta_spqr::State}::from_bytes]: loop 0:
-    Source: 'spqr/src/lib.rs', lines 1013:8-1021:9
+    Source: 'spqr/src/lib.rs', lines 1015:8-1023:9
     Visibility: public -/
 @[rust_loop]
 def State.from_bytes_loop0
@@ -2175,7 +2274,7 @@ def State.from_bytes_loop0
     (iter, pos, chains, chains_ok)
 
 /-- [tacenta_spqr::{tacenta_spqr::State}::from_bytes]: loop body 1:
-    Source: 'spqr/src/lib.rs', lines 1040:8-1048:9
+    Source: 'spqr/src/lib.rs', lines 1042:8-1050:9
     Visibility: public -/
 @[rust_loop_body]
 def State.from_bytes_loop1.body
@@ -2200,7 +2299,7 @@ def State.from_bytes_loop1.body
       ok (cont (iter1, pos1, skipped1, skipped_ok))
 
 /-- [tacenta_spqr::{tacenta_spqr::State}::from_bytes]: loop 1:
-    Source: 'spqr/src/lib.rs', lines 1040:8-1048:9
+    Source: 'spqr/src/lib.rs', lines 1042:8-1050:9
     Visibility: public -/
 @[rust_loop]
 def State.from_bytes_loop1
@@ -2215,7 +2314,7 @@ def State.from_bytes_loop1
     (iter, pos, skipped, skipped_ok)
 
 /-- [tacenta_spqr::{tacenta_spqr::State}::from_bytes]:
-    Source: 'spqr/src/lib.rs', lines 971:4-1074:5
+    Source: 'spqr/src/lib.rs', lines 973:4-1076:5
     Visibility: public -/
 def State.from_bytes
   (bytes : Slice Std.U8) :
